Migrate main sealing file. Remove printing.

sealing/main.v
@@ -3,8 +3,8 @@ TODO: write better testing support -- e.g. comparing final states
 *)
 
 Require Import ssreflect ssrfun eqtype ssrnat ssrbool seq ssrint.
-Require Import ord word.
-Require Import lib.utils common.common.
+Require Import ord word partmap hseq.
+Require Import lib.utils lib.word_utils common.common.
 Require Import concrete.concrete.
 Require Import concrete.int_32.
 Require Import concrete.exec.
@@ -79,171 +79,158 @@ Definition kernel_code {X} l : @relocatable_segment t X w :=
 Instance sk_defs : Sym.sealing_key := {|
  key := [ordType of word 28];
  max_key := monew;
- inc_key := fun x => (x + 1)%w
+ inc_key x := (x + 1)%w;
+ ltb_inc sk := leqw_succ _ sk monew
 |}.
-Proof.
-  rewrite /ordered.ltb /IntOrdered.int_ordered -(lock (IntOrdered.int_ordered_def _))
-          /= /IntOrdered.int_compare /Word.unsigned.
-  intros sk.
-  destruct (equiv_dec sk (Word.repr (Word.max_unsigned 27))) as [H7 | H7]; first by [].
-  rewrite {1 2 3}/Word.ltu.
-  rewrite Word.unsigned_repr //.
-  case: (Coqlib.zlt (Word.unsigned sk) (Word.max_unsigned 27)) => [H6 _ | H6]; last by [].
-  case: (equiv_dec sk (sk + 1)%w) => [|NEQ].
-  { rewrite /= -{1}(Word.add_zero _ sk) => /addwI contra.
-    discriminate. }
-  move: (Word.unsigned_range sk) => [H1' H2'].
-  rewrite addwC -{1 3 5}(add0w sk) Word.translate_ltu //.
-  - rewrite /= /Word.max_unsigned. omega.
-  - have {H7} H7 := H7 : sk <> Word.repr (Word.max_unsigned 27).
-    rewrite [_ 1%w]/=. omega.
-Defined.
 
-Definition encode_sealing_tag (t : Sym.stag) : Word.int 29 :=
+Definition encode_sealing_tag (t : Sym.stag) : word 30 :=
  match t with
-   Sym.DATA => Word.pack [:: 27; 1] [wp Word.zero; Word.zero]%w
- | Sym.KEY k => Word.pack [:: 27; 1] [wp k; Word.one]%w
- | Sym.SEALED k => Word.pack [:: 27; 1] [wp k; Word.repr 3]%w
+   Sym.DATA => @wpack [:: 28; 2] [hseq 0; 0]%w
+ | Sym.KEY k => @wpack [:: 28; 2] [hseq k; 1]%w
+ | Sym.SEALED k => @wpack [:: 28; 2] [hseq k; as_word 3]%w
  end.
 
-Definition decode_sealing_tag (t : Word.int 29) : option Sym.stag :=
-  let: [wu k; t]%w := Word.unpack [:: 27; 1] t in
-  if t == Word.zero then
-    if k == Word.zero then Some Sym.DATA
+Definition decode_sealing_tag (t : word 30) : option Sym.stag :=
+  let: [hseq k; t] := @wunpack [:: 28; 2] t in
+  if t == 0%w then
+    if k == 0%w then Some Sym.DATA
     else None
-  else if t == Word.one then
+  else if t == 1%w then
     Some (Sym.KEY k)
-  else if t == Word.repr 3 then
+  else if t == as_word 3 then
     Some (Sym.SEALED k)
   else None.
 
 Lemma encode_sealing_tagK t : decode_sealing_tag (encode_sealing_tag t) = Some t.
 Proof.
   case: t => [|k|k];
-  by rewrite /decode_sealing_tag /encode_sealing_tag Word.packK /=.
+  by rewrite /decode_sealing_tag /encode_sealing_tag wpackK /=.
 Qed.
 
 Lemma decode_sealing_tagK w t : decode_sealing_tag w = Some t ->
                                 encode_sealing_tag t = w.
 Proof.
   rewrite /decode_sealing_tag /encode_sealing_tag.
-  case E: (Word.unpack [:: 27; 1] w) => [k [w' []]].
-  move: (Word.unpackK [:: 27; 1] w). rewrite E.
-  have [?|?] := altP (w' =P Word.zero); try subst w'.
-  { have [?|?] := altP (k =P Word.zero); try subst k; last by [].
+  case E: (wunpack _) => [k [w' []]].
+  move: (@wunpackK [:: 28; 2] w). rewrite E.
+  have [?|?] := altP (w' =P _); try subst w'.
+  { have [?|?] := altP (k =P _); try subst k; last by [].
     by move => H [<-]. }
-  have [?|?] := altP (w' =P Word.one); try subst w'.
+  have [?|?] := altP (w' =P _); try subst w'.
   { by move => H [<-]. }
-  have [?|?] := altP (w' =P Word.repr 3); try subst w'; last by [].
+  have [?|?] := altP (w' =P _); try subst w'; last by [].
   by move => H [<-].
 Qed.
 
 Instance encodable_tag : @encodable t Sym.stags := {|
   decode k mem w :=
-    let: [wu ut; w']%w := Word.unpack [:: 29; 1] w in
-    if w' == Word.zero then None
+    let: [hseq ut; w'] := @wunpack [:: 30; 2] w in
+    if w' == 0%w then None
     else
       match k with
       | Symbolic.P => Some (USER tt)
       | _ =>
-        if w' == Word.one then
+        if w' == 1%w then
             do! ut <- decode_sealing_tag ut;
             Some (@USER Sym.stag_eqType ut)
-        else if w' == Word.repr 2 then
+        else if w' == as_word 2 then
           do! ut <- decode_sealing_tag ut;
           Some (@ENTRY Sym.stag_eqType ut)
         else None
       end
 |}.
 Proof.
-  - by eauto.
-  - by [].
+  by eauto.
+set ws := wunpack _.
+suff -> : ws = [hseq 0; 0]%w by move=> tk _; rewrite !eqxx.
+rewrite {}/ws /wunpack bits_zero.
+admit.
 Qed.
 
-Definition DATA : word t := Word.repr 0.
+Definition DATA : mword t := 0%w.
 
 Definition transfer_function : list (instr t) :=
  let assert_DATA r := [::
-   Const (Word.casts DATA) ri1;
+   Const (swcast DATA) ri1;
    Binop EQ r ri1 ri1 ] ++
                         if_ ri1 [::] [:: Halt _]
    in
  (* entry points for system calls *)
- ([:: Const (Word.repr (vop_to_Z SERVICE)) ri1;
+ ([:: Const (as_word (nat_of_vop SERVICE)) ri1;
       Binop EQ rop ri1 ri1 ] ++
   (if_ ri1
     [::]
  (* NOP *)
- ([:: Const (Word.repr (op_to_Z NOP)) ri1;
+ ([:: Const (as_word (nat_of_op NOP)) ri1;
       Binop EQ rop ri1 ri1 ] ++
   (if_ ri1
     (assert_DATA rtpc ++ assert_DATA rti ++
-     [:: Const (Word.casts DATA) rtrpc;
-         Const (Word.casts DATA) rtr
+     [:: Const (swcast DATA) rtrpc;
+         Const (swcast DATA) rtr
      ])
  (* CONST *)
- ([:: Const (Word.repr (op_to_Z CONST)) ri1;
+ ([:: Const (as_word (nat_of_op CONST)) ri1;
       Binop EQ rop ri1 ri1 ] ++
   (if_ ri1
     (assert_DATA rtpc ++ assert_DATA rti ++
-     [:: Const (Word.casts DATA) rtrpc;
-         Const (Word.casts DATA) rtr
+     [:: Const (swcast DATA) rtrpc;
+         Const (swcast DATA) rtr
      ])
  (* MOV *)
- ([:: Const (Word.repr (op_to_Z MOV)) ri1;
+ ([:: Const (as_word (nat_of_op MOV)) ri1;
       Binop EQ rop ri1 ri1 ] ++
   (if_ ri1
     (assert_DATA rtpc ++ assert_DATA rti ++
-     [:: Const (Word.casts DATA) rtrpc;
+     [:: Const (swcast DATA) rtrpc;
       Mov rt1 rtr
      ])
  (* BINOPs *)
  (let binop cont b :=
-        [:: Const (Word.repr (op_to_Z (BINOP b))) ri1;
+        [:: Const (as_word (nat_of_op (BINOP b))) ri1;
             Binop EQ rop ri1 ri1 ] ++
         (if_ ri1
           (assert_DATA rtpc ++ assert_DATA rti ++
            assert_DATA rt1 ++ assert_DATA rt2 ++
-           [:: Const (Word.casts DATA) rtrpc;
-               Const (Word.casts DATA) rtr
+           [:: Const (swcast DATA) rtrpc;
+               Const (swcast DATA) rtr
            ])
           cont) in
    foldl binop [::] binops ++
  (* LOAD *)
- ([:: Const (Word.repr (op_to_Z LOAD)) ri1;
+ ([:: Const (as_word (nat_of_op LOAD)) ri1;
       Binop EQ rop ri1 ri1 ] ++
   (if_ ri1
     (assert_DATA rtpc ++ assert_DATA rti ++ assert_DATA rt1 ++
-     [:: Const (Word.casts DATA) rtrpc;
+     [:: Const (swcast DATA) rtrpc;
       Mov rt2 rtr
      ])
  (* STORE *)
- ([:: Const (Word.repr (op_to_Z STORE)) ri1;
+ ([:: Const (as_word (nat_of_op STORE)) ri1;
       Binop EQ rop ri1 ri1 ] ++
   (if_ ri1
     (assert_DATA rtpc ++ assert_DATA rti ++ assert_DATA rt1 ++
-     [:: Const (Word.casts DATA) rtrpc;
+     [:: Const (swcast DATA) rtrpc;
          Mov rt2 rtr
      ])
  (* JUMP *)
- ([:: Const (Word.repr (op_to_Z JUMP)) ri1;
+ ([:: Const (as_word (nat_of_op JUMP)) ri1;
       Binop EQ rop ri1 ri1 ] ++
   (if_ ri1
     (assert_DATA rtpc ++ assert_DATA rti ++
-     [:: Const (Word.casts DATA) rtrpc])
+     [:: Const (swcast DATA) rtrpc])
  (* BNZ *)
- ([:: Const (Word.repr (op_to_Z BNZ)) ri1;
+ ([:: Const (as_word (nat_of_op BNZ)) ri1;
       Binop EQ rop ri1 ri1 ] ++
   (if_ ri1
     (assert_DATA rtpc ++ assert_DATA rti ++ assert_DATA rt1 ++
-     [:: Const (Word.casts DATA) rtrpc])
+     [:: Const (swcast DATA) rtrpc])
  (* JAL *)
- ([:: Const (Word.repr (op_to_Z JAL)) ri1;
+ ([:: Const (as_word (nat_of_op JAL)) ri1;
       Binop EQ rop ri1 ri1 ] ++
   (if_ ri1
     (assert_DATA rtpc ++ assert_DATA rti ++ assert_DATA rt1 ++
-     [:: Const (Word.casts DATA) rtrpc;
-         Const (Word.casts DATA) rtr])
+     [:: Const (swcast DATA) rtrpc;
+         Const (swcast DATA) rtr])
  (* Unknown opcode: Halt *)
  ([:: Halt _])))))))))))))))))))).
 
@@ -251,25 +238,25 @@ Definition fault_handler : @relocatable_segment t w w :=
  kernel_code (fault_handler.handler t fhp transfer_function).
 
 Definition extra_state : @relocatable_segment t w w :=
- kernel_data [:: Word.reprn 13].
+ kernel_data [:: as_word 13].
 
 Definition gen_syscall_code gen : @relocatable_segment t w w :=
- (length (gen (Word.repr 0) (Word.repr 0)),
+ (length (gen (as_word 0) (as_word 0)),
   fun b w => map encode_instr (gen b w)).
 
 Definition mkkey_segment : @relocatable_segment t w w :=
  gen_syscall_code (fun _ (extra : w) =>
-        [:: Const (Word.casts extra) ri1; (* load next key *)
+        [:: Const (swcast extra) ri1; (* load next key *)
             Load ri1 ri5;
-            Const (Word.repr 1) ri3; (* increment and store back *)
+            Const (as_word 1) ri3; (* increment and store back *)
             Binop ADD ri5 ri3 ri3;
             Store ri1 ri3;
-            Const (Word.repr 2) ri3; (* wrap k as KEY(k): SHL by 2 and add 1 *)
+            Const (as_word 2) ri3; (* wrap k as KEY(k): SHL by 2 and add 1 *)
             Binop SHL ri5 ri3 ri4;
-            Const Word.one ri3;
+            Const 1%w ri3;
             Binop ADD ri3 ri4 ri4] ++
         wrap_user_tag ri4 ri4 ++
-        [:: Const Word.zero ri5; (* payload for new key is 0, arbitrarily *)
+        [:: Const 0%w ri5; (* payload for new key is 0, arbitrarily *)
             PutTag ri5 ri4 syscall_ret; (* build the key *)
             Jump ra
          ]).
@@ -280,20 +267,20 @@ Definition seal_segment : @relocatable_segment t w w :=
        [:: GetTag syscall_arg1 ri3] ++
        extract_user_tag ri3 rb ri3 ++
        if_ rb [::] [:: Halt _] ++
-       [:: Const (Word.repr 3) ri5;
+       [:: Const (as_word 3) ri5;
            Binop AND ri3 ri5 ri5] ++
        if_ ri5 [:: Halt _] [::] ++
        (* Ensure that second argument is tagged KEY, halting otherwise *)
        [:: GetTag syscall_arg2 ri4] ++
        extract_user_tag ri4 rb ri4 ++
        if_ rb [::] [:: Halt _] ++
-       [:: Const (Word.repr 3) ri5;
+       [:: Const (as_word 3) ri5;
            Binop AND ri4 ri5 ri2;
-           Const (Word.repr 1) ri5;
+           Const (as_word 1) ri5;
            Binop EQ ri5 ri2 ri5] ++
        if_ ri5 [::] [:: Halt _] ++
        (* Form SEALED(k) tag from KEY(k) in ri4 *)
-       [:: Const (Word.repr 2) ri5;
+       [:: Const (as_word 2) ri5;
            Binop OR ri5 ri4 ri4] ++
        wrap_user_tag ri4 ri4 ++
        [:: PutTag syscall_arg1 ri4 syscall_ret] ++
@@ -301,7 +288,7 @@ Definition seal_segment : @relocatable_segment t w w :=
        [:: GetTag ra ri3] ++
        extract_user_tag ri3 rb ri3 ++
        if_ rb [::] [:: Halt _] ++
-       [:: Const (Word.repr 0) ri5;
+       [:: Const (as_word 0) ri5;
            Binop EQ ri3 ri5 ri5] ++
        if_ ri5 [:: Jump ra] [:: Halt _]
  ).
@@ -312,13 +299,13 @@ Definition unseal_segment : @relocatable_segment t w w :=
        [:: GetTag syscall_arg2 ri4] ++
        extract_user_tag ri4 rb ri4 ++
        if_ rb [::] [:: Halt _] ++
-       [:: Const (Word.repr 3) ri5;
+       [:: Const (as_word 3) ri5;
            Binop AND ri4 ri5 ri2;
-           Const (Word.repr 1) ri5;
+           Const (as_word 1) ri5;
            Binop EQ ri5 ri2 ri5] ++
        if_ ri5 [::] [:: Halt _] ++
        (* Form SEALED(k) tag from KEY(k) in ri4 *)
-       [:: Const (Word.repr 2) ri5;
+       [:: Const (as_word 2) ri5;
            Binop OR ri5 ri4 ri4] ++
        (* Ensure that first argument has a user tag (put it in ri3) *)
        [:: GetTag syscall_arg1 ri3] ++
@@ -328,7 +315,7 @@ Definition unseal_segment : @relocatable_segment t w w :=
        [:: Binop EQ ri3 ri4 ri4] ++
        if_ ri5 [::] [:: Halt _] ++
        (* Retag the payload with DATA *)
-       [:: Const (Word.repr 0) ri5] ++
+       [:: Const (as_word 0) ri5] ++
        wrap_user_tag ri5 ri5 ++
        [:: PutTag syscall_arg1 ri5 syscall_ret] ++
        (* Check that return PC is tagged DATA *)
@@ -337,7 +324,7 @@ Definition unseal_segment : @relocatable_segment t w w :=
        [:: GetTag ra ri3] ++
        extract_user_tag ri3 rb ri3 ++
        if_ rb [::] [:: Halt _] ++
-       [:: Const (Word.repr 0) ri5;
+       [:: Const (as_word 0) ri5;
            Binop EQ ri3 ri5 ri5] ++
        if_ ri5 [:: Jump ra] [:: Halt _]
 ).
@@ -405,28 +392,28 @@ Definition build_symbolic_sealing_machine
                          user_memory_addr@tt
                          ssa
                          user_registers
-                         (common.Atom (Word.repr 0) Sym.DATA)
-                         (Word.repr 0).
+                         (common.Atom (as_word 0) Sym.DATA)
+                         (as_word 0).
 
 (* ---------------------------------------------------------------- *)
 (* ---------------------------------------------------------------- *)
 (* ---------------------------------------------------------------- *)
 (* Abstract machine *)
 
-Definition keytype := [eqType of nat].
+Definition keytype := [ordType of nat].
 
 Definition max_element (l : list keytype) : keytype :=
  foldr maxn O l.
 
 Lemma max_element_plus_one_is_distinct :
- forall (l : list keytype),
+ forall (l : seq keytype),
    1 + max_element l \notin l.
 Proof.
  move => l.
  have MAX: forall x, x \in l -> x <= max_element l.
  { elim: l => [|x' l IH] // x /orP [/eqP -> | THERE] //=.
    - by rewrite leq_max leqnn.
-   - by rewrite leq_max IH //= orb_true_r. }
+   - by rewrite leq_max IH //= orbT. }
  apply/negP => CONTRA.
  move: (MAX _ CONTRA).
  rewrite /addn /addn_rec.
@@ -460,283 +447,28 @@ Definition build_abstract_sealing_machine
     base_addr
     user_registers.
 
-(* ---------------------------------------------------------------- *)
-(* ---------------------------------------------------------------- *)
-(* --------------------------------------------------------------- *)
-(* Printing, mostly ... *)
-
-(* TODO: Some of this belongs elsewhere, like in concrete/int_32 *)
-
-Open Scope Z_scope.
-
-Require Import String.
-Import printing.
-
-Definition format_atom atom :=
-  let: w1@w2 := atom in
-    match decode_instr w1 with
-      Some i => ss "(" +++ format_instr i +++ ss ")@" +++ format_word w2
-    | None => format_word w1 +++ ss "@" +++ format_word w2
-    end.
-
-Definition print_instr (a : atom) :=
-  let: w1@w2 := a in (Word.unsigned w1, decode_instr w1, Word.unsigned w2).
-
-Definition print_atom (a : atom) :=
-  let: w1@w2 := a in (Word.unsigned w1, Word.unsigned w2).
-
-Definition format_mvec l :=
-  let os := match word_to_op (@Concrete.cop (word t) l) with
-              Some o => format_opcode o
-            | None => ss "<BAD OPCODE>"
-            end in
-   os
-   +++ sspace +++
-   format_word (@Concrete.ctpc (word t) l)
-   +++ sspace +++
-   format_word (@Concrete.cti (word t) l)
-   +++ sspace +++
-   format_word (@Concrete.ct1 (word t) l)
-   +++ sspace +++
-   format_word (@Concrete.ct2 (word t) l)
-   +++ sspace +++
-   format_word (@Concrete.ct3 (word t) l).
-
-Definition format_rvec l :=
-   format_word (@Concrete.ctrpc (word t) l)
-   +++ sspace +++
-   format_word (@Concrete.ctr (word t) l).
-
-Definition format_whole_cache (c : Concrete.rules (word t)) :=
-  map (fun l => let: (m,r) := l in (format_mvec m +++ ss " => " +++ format_rvec r)) c.
-
-Definition format_cache (c : Concrete.rules (word t)) :=
-  format_whole_cache (take 3 c).
-
-Fixpoint enum (M R S : Type) s (map : M) (get : M -> Word.int s -> R) (f : R -> S) (n : nat) (i : Word.int s) :=
-  match n with
-  | O => [::]
-  | S p => (Word.unsigned i, f (get map i)) :: enum map get f p (Word.add i (Word.repr 1))
-  end.
-
-Definition summarize_concrete_state mem_count cache_count st :=
-  let mem' := just_somes
-               (@enum _ _ _ _
-                 (@Concrete.mem t st)
-                 (@PartMaps.get _ (word t) (@word_map_class _) _)
-                 (@omap atom sstring format_atom)
-                 mem_count
-                 (Word.repr 0)) in
-  let mem := ssconcat sspace (map (fun x => let: (addr,con) := x in format_Z addr +++ ss ":" +++ con) mem') in
-  let regs' := @enum _ _ _ _
-                 (@Concrete.regs t st)
-                 (@PartMaps.get _ (reg t) (@reg_map_class _) _)
-                 (@omap atom sstring format_atom)
-                 (Z.to_nat (Word.unsigned user_reg_max))
-                 (Word.repr 0) in
-  let regs := map (fun r =>
-                     let: (x,a) := r in
-                     ss "r" +++ format_nat (nat_of_Z x) +++ ss "=" +++
-                        match a with
-                        | Some a => a
-                        | None => ss "_"
-                        end)
-               regs' in
-  let current_instr :=
-    let: addr@_ := Concrete.pc st in
-    match @PartMaps.get _ (word t) _ _
-                    (@Concrete.mem t st)
-                    addr with
-      None => ss "(BAD ADDR)"
-    | Some i => format_atom i
-    end in
-  (to_string
-     (ss "PC=" +++ format_atom (Concrete.pc st) +++ ss "  "
-               +++ current_instr +++
-      ss " | " +++
-      ssconcat sspace regs +++
-      ss " | " +++
-      mem +++
-      ss " | " +++
-      ssconcat sspace (format_whole_cache
-                         (take cache_count (Concrete.cache st))))).
-
-(* ---------------------------------------------------------------- *)
-(* Printing symbolic states *)
-
-Definition format_symbolic_word k (pr_tag : @Symbolic.ttypes (@Sym.sym_sealing sk_defs) k -> sstring) w :=
-    match decode_instr w with
-      Some i => ss "(" +++ format_instr i +++ ss ")"
-    | None => format_word w
-    end.
-
-Definition format_symbolic_atom k (pr_tag : @Symbolic.ttypes (@Sym.sym_sealing sk_defs) k -> sstring) a :=
-  let: w1@t2 := a in
-  format_symbolic_word pr_tag w1 +++ ss "@" +++ pr_tag t2.
-
-Definition summarize_symbolic_state mem_count st pr_tag :=
-  let mem' := just_somes
-               (@enum _ _ _ _
-                 (@Symbolic.mem t Sym.sym_sealing st)
-                 (@PartMaps.get _ (word t) (@word_map_class _) _)
-                 (@omap _ sstring (format_symbolic_atom pr_tag))
-                 mem_count
-                 (Word.repr 0)) in
-  let mem := ssconcat sspace (map (fun x => let: (addr,con) := x in format_Z addr +++ ss ":" +++ con) mem') in
-  let regs' := just_somes
-                 (@enum _ _ _ _
-                    (@Symbolic.regs t Sym.sym_sealing st)
-                    (@PartMaps.get _ (reg t) _ _)
-                    (@omap _ sstring (format_symbolic_atom pr_tag))
-                    (Z.to_nat (Word.unsigned user_reg_max))
-                    (Word.repr 0)) in
-  let regs := map (fun r =>
-                     let: (x,a) := r in
-                     ss "r" +++ format_nat (nat_of_Z x) +++ ss "=" +++ a)
-               regs' in
-  let current_instr :=
-    let: addr := Symbolic.pc st in
-    match @PartMaps.get _ (word t) _ _
-                    (@Symbolic.mem t Sym.sym_sealing st)
-                    (val addr) with
-      None => ss "(BAD ADDR)"
-    | Some i => format_symbolic_atom pr_tag i
-    end in
-  (to_string
-     (ss "PC=" +++ format_symbolic_word pr_tag (val (Symbolic.pc st)) +++ ss "  "
-               +++ current_instr +++
-      ss " | " +++
-      ssconcat sspace regs +++
-      ss " | " +++
-      mem)).
-
-Definition format_int {n} (i : Word.int n) :=
-  format_Z (Word.unsigned i).
-
-Definition format_sealing_tag (t:Sym.stag):=
-  match t with
-    Sym.DATA => ss "DATA"
-  | Sym.KEY k => ss "KEY(" +++ format_int k +++ ss ")"
-  | Sym.SEALED k => ss "SEALED(" +++ format_int k +++ ss ")"
-  end.
-
-Definition summarize_symbolic_sealing_state mem_count st :=
-  summarize_symbolic_state mem_count st format_sealing_tag.
-
-(* ---------------------------------------------------------------- *)
-(* Printing abstract states *)
-
-Definition format_value v :=
-  match v with
-  | Abs.VData w =>
-      match decode_instr w with
-        Some i => ss "(" +++ format_instr i +++ ss ")"
-      | None => format_word w
-      end
-  | Abs.VKey k =>
-      ss "KEY(" +++ format_nat k +++ ss ")"
-  | Abs.VSealed w k =>
-      ss "SEALED(" +++ format_word w +++ ss "," +++ format_nat k +++ ss ")"
-  end.
-
-Definition summarize_abstract_state mem_count st :=
-  let mem' := just_somes
-               (@enum _ _ _ _
-                 (@Abs.mem t sk st)
-                 (@PartMaps.get _ (word t) _ _)
-                 (@omap (@Abs.value t sk) sstring format_value)
-                 mem_count
-                 (Word.repr 0)) in
-  let mem := ssconcat sspace (map (fun x => let: (addr,con) := x in format_Z addr +++ ss ":" +++ con) mem') in
-  let regs' := just_somes
-                 (@enum _ _ _ _
-                    (@Abs.regs t sk st)
-                    (@PartMaps.get _ (reg t) _ _)
-                    (@omap (@Abs.value t sk) sstring format_value)
-                    (Z.to_nat (Word.unsigned user_reg_max))
-                    (Word.repr 0)) in
-  let regs := map (fun r =>
-                     let: (x,a) := r in
-                     ss "r" +++ format_nat (nat_of_Z x) +++ ss "=" +++ a)
-               regs' in
-  let current_instr :=
-    let: addr := Abs.pc st in
-    match @PartMaps.get _ (word t) _ _
-                    (@Abs.mem t sk st)
-                    addr with
-      None => ss "(BAD ADDR)"
-    | Some i => format_value i
-    end in
-  (to_string
-     (ss "PC=" +++ format_word (Abs.pc st) +++ ss "  "
-               +++ current_instr +++
-      ss " | " +++
-      ssconcat sspace regs +++
-      ss " | " +++
-      mem)).
-
-(* ---------------------------------------------------------------- *)
-(* Tests... *)
-
-Definition runn n p :=
-  let init := build_concrete_sealing_machine p in
-  let tr := utils.runn (@step masks t _) n init in
-  (
-   summarize_concrete_state 3000 1000 init ::
-   map (summarize_concrete_state 8 1) tr
-  ).
-
-Definition run := runn 10000.
-
-Definition run_abs n p :=
-  let init := build_abstract_sealing_machine p in
-  let '(_,_,syscall_addrs) := concrete_sealing_monitor in
-  let tr := utils.runn (fun x => Abs.stepf x) n init in
-  (
-   summarize_abstract_state 3000 init ::
-   map (summarize_abstract_state 8) tr
-  ).
-
-
-Definition run_sym n p :=
-  let init := build_symbolic_sealing_machine p in
-  let '(_,_,syscall_addrs) := concrete_sealing_monitor in
-  let tr := utils.runn (fun x => @stepf concrete_int_32_t concrete_int_32_ops
-                                 (@Sym.sym_sealing sk_defs)
-                                 Sym.sealing_syscalls
-                                 x) n init in
-  (
-   summarize_symbolic_sealing_state 3000 init ::
-   map (summarize_symbolic_sealing_state 8) tr
-  ).
-
-(* BCP: TODO: Arguably the second argument to f should be a list of
-   imm'ediates, not words... *)
-(* AAA: TODO: Do we still need user code to take system call address
-   as its parameters? After all, we now know all of them. *)
 Definition user_code (f : w -> @classes.sealing_syscall_addrs t -> list (instr t))
                   : @relocatable_segment t (@classes.sealing_syscall_addrs t) (instr t) :=
- (List.length (f user_memory_addr ssa),
-  f).
+ (size (f user_memory_addr ssa), f).
 
 Definition hello_world0 : @relocatable_segment t (@classes.sealing_syscall_addrs t) (instr concrete_int_32_t) :=
   user_code (fun _ _ => [::
-     Const (Word.repr 2) ruser1
+     Const (as_word 2) ruser1
   ]).
 
 Definition hello_world1 : @relocatable_segment t (@classes.sealing_syscall_addrs t) (instr concrete_int_32_t) :=
   user_code (fun _ _ => [::
-    Const (Word.repr 2) ruser1;
+    Const (as_word 2) ruser1;
     Binop ADD ruser1 ruser1 ruser2
   ]).
 
 Definition hello_world2 : @relocatable_segment t (@classes.sealing_syscall_addrs t) (instr t) :=
   user_code (fun _ _ =>
         [::
-          Const (Word.casts classes.mkkey_addr) ruser1;
+          Const (swcast classes.mkkey_addr) ruser1;
           Jal ruser1;
-          Const (Word.casts classes.seal_addr) ruser1;
-          Const (Word.repr 17) syscall_arg1;
+          Const (swcast classes.seal_addr) ruser1;
+          Const (as_word 17) syscall_arg1;
           Mov syscall_ret syscall_arg2;
           Jal ruser1
         ]
@@ -746,10 +478,10 @@ Definition hello_world2 : @relocatable_segment t (@classes.sealing_syscall_addrs
 Definition hello_world3 : @relocatable_segment t (@classes.sealing_syscall_addrs t) (instr concrete_int_32_t) :=
   user_code (fun _ _ =>
         [::
-          Const (Word.casts classes.mkkey_addr) ruser1;
+          Const (swcast classes.mkkey_addr) ruser1;
           Jal ruser1;
-          Const (Word.casts classes.seal_addr) ruser1;
-          Const (Word.repr 17) syscall_arg1;
+          Const (swcast classes.seal_addr) ruser1;
+          Const (as_word 17) syscall_arg1;
           Mov syscall_ret syscall_arg2;
           Jal ruser1;
           Mov syscall_ret syscall_arg1;
@@ -761,14 +493,14 @@ Definition hello_world3 : @relocatable_segment t (@classes.sealing_syscall_addrs
 Definition hello_world4 : @relocatable_segment t (@classes.sealing_syscall_addrs t) (instr concrete_int_32_t) :=
   user_code (fun _ _ =>
         [::
-          Const (Word.casts classes.mkkey_addr) ruser1;
+          Const (swcast classes.mkkey_addr) ruser1;
           Jal ruser1;
           Mov syscall_ret syscall_arg2;
-          Const (Word.casts classes.seal_addr) ruser1;
-          Const (Word.repr 17) syscall_arg1;
+          Const (swcast classes.seal_addr) ruser1;
+          Const (as_word 17) syscall_arg1;
           Jal ruser1;
           Mov syscall_ret syscall_arg1;
-          Const (Word.casts classes.unseal_addr) ruser1;
+          Const (swcast classes.unseal_addr) ruser1;
           Jal ruser1
         ]
   ).
@@ -776,16 +508,16 @@ Definition hello_world4 : @relocatable_segment t (@classes.sealing_syscall_addrs
 (* Test store and load *)
 Definition hello_world5 : @relocatable_segment t (@classes.sealing_syscall_addrs t) (instr concrete_int_32_t) :=
   user_code (fun base _ =>
-    let data := Word.casts (Word.add base (Word.repr 0)) in
+    let data := swcast (base + 0)%w in
         [::
           (* DATA BLOCK *)
           Nop _;
           (* As before, make up a key and seal 17 with it *)
-          Const (Word.casts classes.mkkey_addr) ruser1;
+          Const (swcast classes.mkkey_addr) ruser1;
           Jal ruser1;
           Mov syscall_ret syscall_arg2;
-          Const (Word.casts classes.seal_addr) ruser1;
-          Const (Word.repr 17) syscall_arg1;
+          Const (swcast classes.seal_addr) ruser1;
+          Const (as_word 17) syscall_arg1;
           Jal ruser1;
           (* Store it in the data block and read it back *)
           Const data ruser1;
@@ -793,14 +525,6 @@ Definition hello_world5 : @relocatable_segment t (@classes.sealing_syscall_addrs
           Load ruser1 ruser2
         ]
   ).
-
-(* Run tests like this:
-
-Concrete Machine: Compute (runn 2000 hello_world5).
-
-Symbolic Machine: Compute (run_sym 2000 hello_world5).
-
-Abstract Machine: Compute (run_abs 2000 hello_world5). *)
 
 Section Refinement.
 
@@ -815,12 +539,12 @@ Context {implementation_correct : kernel_code_bwd_correctness monitor_invariant 
 Inductive refine_state (ast : Abs.state t) (cst : Concrete.state t) : Prop :=
 | rs_intro : forall sst m,
                refinement_common.refine_state monitor_invariant Sym.sealing_syscalls sst cst ->
-               @refinementSA.refine_state t sk_defs sk _ nat_partial_map m ast sst ->
+               @refinementSA.refine_state t sk_defs sk m ast sst ->
                refine_state ast cst.
 Hint Constructors refine_state.
 
-Lemma backwards_refinement_as ast sst sst' (m : NatPMap.t _) :
-  @refinementSA.refine_state t sk_defs sk _ nat_partial_map m ast sst ->
+Lemma backwards_refinement_as ast sst sst' m :
+  @refinementSA.refine_state t sk_defs sk m ast sst ->
   exec (Symbolic.step Sym.sealing_syscalls) sst sst' ->
   exists ast' m',
     exec (fun ast ast' => Abs.step ast ast') ast ast' /\
@@ -828,9 +552,9 @@ Lemma backwards_refinement_as ast sst sst' (m : NatPMap.t _) :
 Proof.
   move => REF EXEC.
   elim: EXEC ast m REF => {sst sst'} [sst _ |sst sst' sst'' _ STEPS EXEC IH] ast m REF; first by eauto 7.
-  exploit refinementSA.backward_simulation; eauto.
+  generalize (refinementSA.backward_simulation REF STEPS).
   intros (ast' & m' & STEPA & REF').
-  exploit IH; eauto.
+  have := IH _ _ REF'.
   intros (ast'' & m'' & EXECA & REF''). by eauto 7.
 Qed.
 
@@ -843,9 +567,8 @@ Lemma backwards_refinement ast cst cst' :
     refine_state ast' cst'.
 Proof.
   move => [sst m SC AS] EXECC INUSER.
-  generalize (backwards_refinement SC EXECC INUSER).
-  move => [sst' [EXECS SC']].
-  exploit backwards_refinement_as; eauto.
+  generalize (backwards_refinement SC EXECC INUSER) => - [sst' EXECS SC'].
+  have := backwards_refinement_as AS EXECS.
   intros (ast' & m' & EXECA & AS'). by eauto 7.
 Qed.
 
